iris/ProofKwait.v
@@ -882,7 +882,7 @@ Section ProofKwait.
     arm_pay KT1 0 eb pme -∗
     kernel_text -∗
     pc_is (mword_of_int (KW + 0xfa)) -∗
-    is_lock γw wait_lock_addr "wait_lock"%string <{ wait_res }> -∗
+    is_lock γw wait_lock_addr "wait_lock"%string wait_res_at -∗
     locked γw CIDt -∗
     wait_res -∗
     kw_frame sp0 mm -∗
@@ -964,7 +964,7 @@ Section ProofKwait.
                      (sign_extend' 64 (mword_of_int 0 : mword 12)) = wait_lock_addr)
       by (rewrite HT2a0; apply addv_sext0).
     (* ---- release(&wait_lock): level 1 -> 0, so the exit index is [eb] ---- *)
-    iApply (Release.wp_release_sconf KT1 γw wait_lock_addr "wait_lock"%string <{ wait_res }> T2 0%nat eb pme (K - 10)%nat _ Hlka ltac:(pose proof (kw_K10 K HK); lia)
+    iApply (Release.wp_release_sconf KT1 γw wait_lock_addr "wait_lock"%string wait_res_at T2 0%nat eb pme (K - 10)%nat _ Hlka ltac:(pose proof (kw_K10 K HK); lia)
               with "Hcg Htext Hpc Hlk Htok Hres Hown Hpay").
     iIntros (CIDr Hsr mr) "Hcg Hpc %Hcsr Hown".
     iEval (rewrite (locks_add_del_below "wait_lock" lks Hbelow)) in "Hown".
@@ -1041,7 +1041,7 @@ Section ProofKwait.
     is_lock γk (proc_addr k) "proc"%string (proc_lock_pay γs γk (proc_addr k)) -∗
     locked γk CIDt -∗
     proc_lock_res γs γk (proc_addr k) -∗
-    is_lock γw wait_lock_addr "wait_lock"%string <{ wait_res }> -∗
+    is_lock γw wait_lock_addr "wait_lock"%string wait_res_at -∗
     locked γw CIDt -∗
     wait_res -∗
     kw_frame sp0 mm -∗
@@ -1188,7 +1188,7 @@ Section ProofKwait.
     assert (Hlkw : add_vec (U4 !!! Regidx Ra0)
                      (sign_extend' 64 (mword_of_int 0 : mword 12)) = wait_lock_addr)
       by (rewrite HU4a0; apply addv_sext0).
-    iApply (Release.wp_release_sconf KT1 γw wait_lock_addr "wait_lock"%string <{ wait_res }> U4 0%nat eb pme (K - 10)%nat _ Hlkw ltac:(pose proof (kw_K10 K HK); lia)
+    iApply (Release.wp_release_sconf KT1 γw wait_lock_addr "wait_lock"%string wait_res_at U4 0%nat eb pme (K - 10)%nat _ Hlkw ltac:(pose proof (kw_K10 K HK); lia)
               with "Hcg Htext Hpc Hlk Htok Hres Hown Hpay0").
     iIntros (CIDr2 Hsr2 mr) "Hcg Hpc %Hcsr Hown".
     iEval (rewrite (locks_add_del_below "wait_lock" lks Hbelow)) in "Hown".
@@ -1282,7 +1282,7 @@ Section ProofKwait.
        ([ProcAvail.v]).  Persistent. *)
     pslot_used_at (proc_addr k) -∗
     (* wait_lock, contents out *)
-    is_lock γw wait_lock_addr "wait_lock"%string <{ wait_res }> -∗
+    is_lock γw wait_lock_addr "wait_lock"%string wait_res_at -∗
     locked γw CIDp -∗
     parents_own ps -∗
     kw_frame sp0 mm -∗
@@ -1542,7 +1542,7 @@ Section ProofKwait.
     assert (Hlkw : add_vec (R6 !!! Regidx Ra0)
                      (sign_extend' 64 (mword_of_int 0 : mword 12)) = wait_lock_addr)
       by (rewrite HR6a0; apply addv_sext0).
-    iApply (Release.wp_release_sconf KT1 γw wait_lock_addr "wait_lock"%string <{ wait_res }> R6 0%nat eb pme (K - 10)%nat _ Hlkw ltac:(pose proof (kw_K10 K HK); lia)
+    iApply (Release.wp_release_sconf KT1 γw wait_lock_addr "wait_lock"%string wait_res_at R6 0%nat eb pme (K - 10)%nat _ Hlkw ltac:(pose proof (kw_K10 K HK); lia)
               with "Hcg Htext Hpc Hlk Htok [Hps] Hown Hpay0").
     { iExists (<[k := (zero_reg : mword 64)]> ps). iExact "Hps". }
     iIntros (CIDr2 Hsr2 mr) "Hcg Hpc %Hcsr Hown".
@@ -1607,7 +1607,7 @@ Section ProofKwait.
        its lock invariant carries it and the rebuild below owes it back
        ([ProcAvail.v]).  Persistent. *)
     pslot_used_at (proc_addr k) -∗
-    is_lock γw wait_lock_addr "wait_lock"%string <{ wait_res }> -∗
+    is_lock γw wait_lock_addr "wait_lock"%string wait_res_at -∗
     locked γw CIDf -∗
     parents_own ps -∗
     proc_priv γf pme pid V -∗
@@ -1997,7 +1997,7 @@ Section ProofKwait.
     procs_inv γs -∗
     kernel_text -∗
     kalloc_env γa None -∗
-    is_lock γw wait_lock_addr "wait_lock"%string <{ wait_res }> -∗
+    is_lock γw wait_lock_addr "wait_lock"%string wait_res_at -∗
     ∀ (kk : nat) (M : regfile) (hv : mword 64) (ps : list (mword 64)),
       ⌜(kk < NPROC)%nat⌝ -∗ ⌜kw_scan_regs M mm pme addr kk⌝ -∗
       ⌜M !!! Regidx Ra4 = hv⌝ -∗
@@ -2465,7 +2465,7 @@ Section ProofKwait.
        reaches. *)
     locks_below lks "wait_lock" ->
     kernel_text -∗
-    is_lock γw wait_lock_addr "wait_lock"%string <{ wait_res }> -∗
+    is_lock γw wait_lock_addr "wait_lock"%string wait_res_at -∗
     kw_exit_fn CIDt γf mm pme K eb pid V lks -∗
     sie_cap_gpr KT1 Mt (trap_res eb + (K - 10))%nat false pme -∗
     cpu_own 1 eb pme false ({["wait_lock"]} ∪ lks) -∗
@@ -2479,7 +2479,7 @@ Section ProofKwait.
     iIntros "#Htext #Hlk Hqfn Hcg Hown Hpay Hpc Htok Hps Hpriv Hframe".
     iApply (kw_exit_wait γw mm Mt pme K eb lks HK Hsp Hcs Hbelow
               with "Hcg Hown Hpay Htext Hpc Hlk Htok [Hps] Hframe [Hqfn Hpriv]").
-    { rewrite /wait_res. iExists px. iExact "Hps". }
+    { rewrite /wait_res /wait_res_at. iExists px. iExact "Hps". }
     rewrite /kw_exit_fn.
     iIntros (CIDx Hsx mf) "%Hcsx %Ha0x Hcgx Hownx Hpcx".
     iSpecialize ("Hqfn" $! CIDx with "[%]"); [exact Hsx |].
@@ -2522,7 +2522,7 @@ Section ProofKwait.
        off this premise. *)
     locks_below lks "wait_lock" ->
     kernel_text -∗ procs_inv γs -∗
-    is_lock γw wait_lock_addr "wait_lock"%string <{ wait_res }> -∗
+    is_lock γw wait_lock_addr "wait_lock"%string wait_res_at -∗
     kw_round CID0 γf γw jj mm pme addr K eb pid V lks -∗
     kw_exit_fn CIDt γf mm pme K eb pid V lks -∗
     sie_cap_gpr KT1 Mx (trap_res eb + (K - 10))%nat false pme -∗
@@ -2763,10 +2763,10 @@ Section ProofKwait.
                          (sign_extend' 64 (mword_of_int 0 : mword 12)) = wait_lock_addr)
           by (rewrite HT5a0; apply addv_sext0).
         (* -------------------- release(&wait_lock) -------------------- *)
-        iApply (Release.wp_release_sconf KT1 γw wait_lock_addr "wait_lock"%string <{ wait_res }> T5 0%nat eb (proc_addr jj) (K - 10)%nat _ Hlka
+        iApply (Release.wp_release_sconf KT1 γw wait_lock_addr "wait_lock"%string wait_res_at T5 0%nat eb (proc_addr jj) (K - 10)%nat _ Hlka
                   ltac:(pose proof (kw_K10 K HK); lia)
                   with "Hcg Htext Hpc Hlk Htok [Hps] Hown Hpay").
-        { rewrite /wait_res. iExists px. iExact "Hps". }
+        { rewrite /wait_res /wait_res_at. iExists px. iExact "Hps". }
         iIntros (CIDr Hsr mfr) "Hcg Hpc %Hrcs Hown".
         iEval (rewrite (locks_add_del_below "wait_lock" lks Hbelow)) in "Hown".
         assert (Hpe4 : ret_pc (T5 !!! Regidx Rra) = mword_of_int (KW + 0xe4))
@@ -2860,7 +2860,7 @@ Section ProofKwait.
         (* -------------------- acquire(&wait_lock) -------------------- *)
         iDestruct (cpu_own_transport CIDs CIDn 0 eb (proc_addr jj) eb
                      ltac:(wp_next_chain) with "Hown") as "Hown".
-        iApply (Acquire.wp_acquire_sconf KT1 γw "wait_lock"%string <{ wait_res }> T8
+        iApply (Acquire.wp_acquire_sconf KT1 γw "wait_lock"%string wait_res_at T8
                   0%nat eb (proc_addr jj) (K - 10)%nat eb lks
                   kw_ilvl0 ltac:(pose proof (kw_K10 K HK); lia) Hbelow
                   with "Hcg Hown Htext Hpc []").
@@ -2909,7 +2909,7 @@ Section ProofKwait.
     locks_below lks "wait_lock" ->
     kernel_text -∗ procs_inv γs -∗
     kalloc_env γa None -∗
-    is_lock γw wait_lock_addr "wait_lock"%string <{ wait_res }> -∗
+    is_lock γw wait_lock_addr "wait_lock"%string wait_res_at -∗
     ▷ kw_round CID0 γf γw jj mm pme addr K eb pid V lks -∗
     kw_exit_fn CIDy γf mm pme K eb pid V lks -∗
     sie_cap_gpr KT1 M (trap_res eb + (K - 10))%nat false pme -∗
@@ -3405,7 +3405,7 @@ Section ProofKwaitMain.
       by (rewrite /P7; apply kw_cs_rest_ncs; [vm_compute; reflexivity | exact HP6cs]).
     iDestruct (cpu_own_transport CID14 CID18 0%nat eb pj eb ltac:(wp_next_chain)
                  with "Hown") as "Hown".
-    iApply (Acquire.wp_acquire_sconf KT1 γw "wait_lock"%string <{ wait_res }> P7 0%nat eb pj
+    iApply (Acquire.wp_acquire_sconf KT1 γw "wait_lock"%string wait_res_at P7 0%nat eb pj
               (av - 10)%nat eb lks kw_ilvl0 ltac:(pose proof (kw_K10 av Hav); lia) Hbelow
               with "Hcg Hown Htext Hpc [Hlk]").
     all: try lkbelow.
